\documentclass{article}
\usepackage{amsmath}

\begin{document}

\title{Stretch-Exponential Approximation}
\author{}
\date{}
\maketitle

\section{Mathematical Derivation}

The given function is:

\[
S(t) = S_0 \exp \left( -\left( \frac{t}{\tau} \right)^b \right)
\]

Taking the natural logarithm:

\[
\ln S = \ln S_0 - \left( \frac{t}{\tau} \right)^b
\]

Define:

\[
\chi = \ln \frac{t}{\tau}
\]

Then:

\[
\left( \frac{t}{\tau} \right)^b = e^{b \chi}
\]

Using the Taylor series expansion:

\[
e^{b \chi} = 1 + b \chi + \frac{b^2}{2} \chi^2 + \frac{b^3}{6} \chi^3 + O(\chi^4)
\]

Thus:

\[
\ln S = \ln S_0 - \left[ 1 + b \chi + \frac{b^2}{2} \chi^2 + \frac{b^3}{6} \chi^3 \right] + O(\chi^4)
\]

Expanding further:

\[
\ln S = \ln S_0 - 1 - b \ln \epsilon + b \ln \tau - \frac{b^2}{2} (\ln \epsilon)^2 + \frac{b^2}{2} (\ln \tau)^2 - \frac{b^3}{6} (\ln \epsilon)^3 + \frac{b^3}{2} \ln \epsilon (\ln \tau)^2 - \frac{b^3}{6} (\ln \tau)^3 + O(\ln \epsilon^4)
\]

Rewriting in terms of coefficients:

\[
\ln S = A_0 + A_1 \ln \epsilon + A_2 (\ln \epsilon)^2 + A_3 (\ln \epsilon)^3 + O(\ln \epsilon^4)
\]

Where:

\[
A_0 = \ln S_0 - 1 + b \ln \tau - \frac{b^2}{2} \ln \tau + \frac{b^2}{2} (\ln \tau)^2
\]

\[
A_1 = -b + b \ln \tau - \frac{b^2}{2} (\ln \tau)^2
\]

\[
A_2 = -\frac{b^2}{2} + \frac{b^3}{2} \ln \tau
\]

\[
A_3 = -\frac{b^3}{6}
\]

Solving for \( b \):

\[
b = (b A_3)^{\frac{1}{3}}
\]

\[
\ln \tau = 2 \left( A_2 + \frac{b^2}{2} \right) b^{-3}
\]

\[
\ln S_0 = A_0 + 1 - b \ln \tau + \frac{b^2}{2} (\ln \tau)^2
\]

\end{document}
